src/Wrapper.v
@@ -50,41 +50,39 @@ Module WMod.
         end.
 
     Definition interp_fun (f: function m.(state) m.(ident) m.(mident))
-      : ktree (((@eventE interp_ident) +' cE) +' sE interp_state) Any.t Any.t :=
-      Mod.wrap_fun
-        (fun (arg: f.(A)) =>
-           _ <- trigger Yield;;
+      : ktree (((@eventE interp_ident) +' cE) +' sE interp_state) f.(A) f.(R) :=
+      fun (arg: f.(A)) =>
+        _ <- trigger Yield;;
 
-           tid <- trigger (GetTid);;
-           '(st, ts) <- trigger (@Get _);;
-           let ts := NatMap.add tid f.(type) ts in
-           _ <- trigger (Put (st, ts));;
-           _ <- trigger (Fair (sum_fmap_l (fun i => if tid_dec i tid then Flag.success else Flag.emp)));;
+        tid <- trigger (GetTid);;
+        '(st, ts) <- trigger (@Get _);;
+        let ts := NatMap.add tid f.(type) ts in
+        _ <- trigger (Put (st, ts));;
+        _ <- trigger (Fair (sum_fmap_l (fun i => if tid_dec i tid then Flag.success else Flag.emp)));;
 
-           ITree.iter
-             (fun (_: unit) =>
-                b <- trigger (Choose bool);;
-                if (b: bool)
-                then
-                  _ <- trigger (Fair (sum_fmap_l (fun i => if tid_dec i tid then Flag.fail else Flag.emp)));;
-                  _ <- trigger Yield;; Ret (inl tt)
-                else
-                  '(st, ts) <- trigger (@Get _);;
-                  next <- trigger (Choose (sig (f.(body) arg st)));;
-                  match proj1_sig next with
-                  | normal st r fm =>
-                      let ts := NatMap.remove tid ts in
-                      _ <- trigger (Fair (interp_fmap fm ts));;
-                      _ <- trigger (Put (st, ts));;
-                      _ <- trigger Yield;;
-                      Ret (inr r)
-                  | stuck _ _ _ _ => UB
-                  | disabled _ _ _ _ => _ <- trigger Yield;; Ret (inl tt)
-                  end) tt)
+        ITree.iter
+          (fun (_: unit) =>
+             b <- trigger (Choose bool);;
+             if (b: bool)
+             then
+               _ <- trigger (Fair (sum_fmap_l (fun i => if tid_dec i tid then Flag.fail else Flag.emp)));;
+               _ <- trigger Yield;; Ret (inl tt)
+             else
+               '(st, ts) <- trigger (@Get _);;
+               next <- trigger (Choose (sig (f.(body) arg st)));;
+               match proj1_sig next with
+               | normal st r fm =>
+                   let ts := NatMap.remove tid ts in
+                   _ <- trigger (Fair (interp_fmap fm ts));;
+                   _ <- trigger (Put (st, ts));;
+                   _ <- trigger Yield;;
+                   Ret (inr r)
+               | stuck _ _ _ _ => UB
+               | disabled _ _ _ _ => _ <- trigger Yield;; Ret (inl tt)
+               end) tt
     .
 
-    Definition interp_fun_register (i: m.(ident)): itree (((@eventE interp_ident) +' cE) +' sE interp_state) unit :=
-      tid <- trigger (GetTid);;
+    Definition interp_fun_register (tid: thread_id) (i: m.(ident)): itree (((@eventE interp_ident) +' cE) +' sE interp_state) unit :=
       '(st, ts) <- trigger (@Get _);;
       let ts := NatMap.add tid i ts in
       _ <- trigger (Put (st, ts));;
@@ -92,14 +90,14 @@ Module WMod.
       Ret tt
     .
 
-    Definition interp_fun_body R (tid: thread_id) (i: m.(ident))
+    Definition interp_fun_body R (tid: thread_id)
                (step: m.(state) -> output m.(state) m.(ident) m.(mident) R -> Prop)
       : itree (((@eventE interp_ident) +' cE) +' sE interp_state) R :=
       ITree.iter
         (fun (_: unit) =>
            b <- trigger (Choose bool);;
            if (b: bool) then
-             _ <- trigger (Fair (sum_fmap_l (fun i => if tid_dec i tid then Flag.success else Flag.emp)));;
+             _ <- trigger (Fair (sum_fmap_l (fun i => if tid_dec i tid then Flag.fail else Flag.emp)));;
              _ <- trigger Yield;; Ret (inl tt)
            else
              '(st, ts) <- trigger (@Get _);;
@@ -115,10 +113,52 @@ Module WMod.
              | disabled _ _ _ _ => _ <- trigger Yield;; Ret (inl tt)
              end) tt.
 
+    Lemma interp_fun_unfold f arg
+      :
+      interp_fun f arg
+      =
+        _ <- trigger Yield;;
+        tid <- trigger (GetTid);;
+        _ <- (interp_fun_register tid f.(type));;
+        interp_fun_body tid (f.(body) arg)
+    .
+    Proof.
+      unfold interp_fun, interp_fun_register, interp_fun_body. grind.
+    Qed.
+
+    Lemma interp_loop_unfold
+          R (tid: thread_id)
+          (step: m.(state) -> output m.(state) m.(ident) m.(mident) R -> Prop)
+      :
+      interp_fun_body tid step
+      =
+        b <- trigger (Choose bool);;
+        if (b: bool) then
+          _ <- trigger (Fair (sum_fmap_l (fun i => if tid_dec i tid then Flag.fail else Flag.emp)));;
+          _ <- trigger Yield;;
+          tau;; interp_fun_body tid step
+        else
+          '(st, ts) <- trigger (@Get _);;
+          next <- trigger (Choose (sig (step st)));;
+          match proj1_sig next with
+          | normal st r fm =>
+              let ts := NatMap.remove tid ts in
+              _ <- trigger (Fair (interp_fmap fm ts));;
+              _ <- trigger (Put (st, ts));;
+              _ <- trigger Yield;;
+              Ret r
+          | stuck _ _ _ _ => UB
+          | disabled _ _ _ _ => _ <- trigger Yield;; tau;; interp_fun_body tid step
+          end.
+    Proof.
+      unfold interp_fun_body at 1. rewrite unfold_iter.
+      unfold interp_fun_body, UB. grind.
+    Qed.
+
     Definition interp_mod: Mod.t :=
       Mod.mk
         (m.(st_init), NatMap.empty m.(ident))
-        (Mod.get_funs (List.map (fun '(fn, f) => (fn, interp_fun f)) m.(funs)))
+        (Mod.get_funs (List.map (fun '(fn, f) => (fn, Mod.wrap_fun (interp_fun f))) m.(funs)))
     .
   End INTERP.
 End WMod.
